heap_lang/notation.v
@@ -28,6 +28,7 @@ Notation "% l" := (Loc l) (at level 8, format "% l") : expr_scope.
 
 Notation "' x" := (Var x) (at level 8, format "' x") : expr_scope.
 Notation "^ v" := (of_val' v%V) (at level 8, format "^ v") : expr_scope.
+Notation "^^ e" := (wexpr' e%E) (at level 8, format "^^ e") : expr_scope.
 
 (** Syntax inspired by Coq/Ocaml. Constructions with higher precedence come
     first. *)
